feat: `TransOrd`, `LawfulOrd`, `BEqOrd` + instances (#730)
Co-authored-by: François G. Dorais <fgdorais@gmail.com>

Std/Classes/Order.lean
@@ -3,13 +3,30 @@ Copyright (c) 2022 Mario Carneiro. All rights reserved.
 Released under Apache 2.0 license as described in the file LICENSE.
 Authors: Mario Carneiro
 -/
+import Std.Tactic.SeqFocus
 
 /-! ## Ordering -/
 
-@[simp] theorem Ordering.swap_swap {o : Ordering} : o.swap.swap = o := by cases o <;> rfl
+namespace Ordering
 
-@[simp] theorem Ordering.swap_inj {o₁ o₂ : Ordering} : o₁.swap = o₂.swap ↔ o₁ = o₂ :=
+@[simp] theorem swap_swap {o : Ordering} : o.swap.swap = o := by cases o <;> rfl
+
+@[simp] theorem swap_inj {o₁ o₂ : Ordering} : o₁.swap = o₂.swap ↔ o₁ = o₂ :=
   ⟨fun h => by simpa using congrArg swap h, congrArg _⟩
+
+theorem swap_then (o₁ o₂ : Ordering) : (o₁.then o₂).swap = o₁.swap.then o₂.swap := by
+  cases o₁ <;> rfl
+
+theorem then_eq_lt {o₁ o₂ : Ordering} : o₁.then o₂ = lt ↔ o₁ = lt ∨ o₁ = eq ∧ o₂ = lt := by
+  cases o₁ <;> cases o₂ <;> decide
+
+theorem then_eq_eq {o₁ o₂ : Ordering} : o₁.then o₂ = eq ↔ o₁ = eq ∧ o₂ = eq := by
+  cases o₁ <;> simp [«then»]
+
+theorem then_eq_gt {o₁ o₂ : Ordering} : o₁.then o₂ = gt ↔ o₁ = gt ∨ o₁ = eq ∧ o₂ = gt := by
+  cases o₁ <;> cases o₂ <;> decide
+
+end Ordering
 
 namespace Std
 
@@ -28,6 +45,8 @@ namespace OrientedCmp
 
 theorem cmp_eq_gt [OrientedCmp cmp] : cmp x y = .gt ↔ cmp y x = .lt := by
   rw [← Ordering.swap_inj, symm]; exact .rfl
+
+theorem cmp_ne_gt [OrientedCmp cmp] : cmp x y ≠ .gt ↔ cmp y x ≠ .lt := not_congr cmp_eq_gt
 
 theorem cmp_eq_eq_symm [OrientedCmp cmp] : cmp x y = .eq ↔ cmp y x = .eq := by
   rw [← Ordering.swap_inj, symm]; exact .rfl
@@ -94,6 +113,247 @@ instance [inst : OrientedCmp cmp] : OrientedCmp (flip cmp) where
 instance [inst : TransCmp cmp] : TransCmp (flip cmp) where
   le_trans h1 h2 := inst.le_trans h2 h1
 
+/-- `BEqCmp cmp` asserts that `cmp x y = .eq` and `x == y` coincide. -/
+class BEqCmp [BEq α] (cmp : α → α → Ordering) : Prop where
+  /-- `cmp x y = .eq` holds iff `x == y` is true. -/
+  cmp_iff_beq : cmp x y = .eq ↔ x == y
+
+theorem BEqCmp.cmp_iff_eq [BEq α] [LawfulBEq α] [BEqCmp (α := α) cmp] : cmp x y = .eq ↔ x = y := by
+  simp [BEqCmp.cmp_iff_beq]
+
+/-- `LTCmp cmp` asserts that `cmp x y = .lt` and `x < y` coincide. -/
+class LTCmp [LT α] (cmp : α → α → Ordering) extends OrientedCmp cmp : Prop where
+  /-- `cmp x y = .lt` holds iff `x < y` is true. -/
+  cmp_iff_lt : cmp x y = .lt ↔ x < y
+
+theorem LTCmp.cmp_iff_gt [LT α] [LTCmp (α := α) cmp] : cmp x y = .gt ↔ y < x := by
+  rw [OrientedCmp.cmp_eq_gt, LTCmp.cmp_iff_lt]
+
+/-- `LECmp cmp` asserts that `cmp x y ≠ .gt` and `x ≤ y` coincide. -/
+class LECmp [LE α] (cmp : α → α → Ordering) extends OrientedCmp cmp : Prop where
+  /-- `cmp x y ≠ .gt` holds iff `x ≤ y` is true. -/
+  cmp_iff_le : cmp x y ≠ .gt ↔ x ≤ y
+
+theorem LTCmp.cmp_iff_ge [LE α] [LECmp (α := α) cmp] : cmp x y ≠ .lt ↔ y ≤ x := by
+  rw [← OrientedCmp.cmp_ne_gt, LECmp.cmp_iff_le]
+
+/-- `LawfulCmp cmp` asserts that the `LE`, `LT`, `BEq` instances are all coherent with each other
+and with `cmp`, describing a strict weak order (a linear order except for antisymmetry). -/
+class LawfulCmp [LE α] [LT α] [BEq α] (cmp : α → α → Ordering) extends
+  TransCmp cmp, BEqCmp cmp, LTCmp cmp, LECmp cmp : Prop
+
+/-- `OrientedOrd α` asserts that the `Ord` instance satisfies `OrientedCmp`. -/
+abbrev OrientedOrd (α) [Ord α] := OrientedCmp (α := α) compare
+
+/-- `TransOrd α` asserts that the `Ord` instance satisfies `TransCmp`. -/
+abbrev TransOrd (α) [Ord α] := TransCmp (α := α) compare
+
+/-- `BEqOrd α` asserts that the `Ord` and `BEq` instances are coherent via `BEqCmp`. -/
+abbrev BEqOrd (α) [BEq α] [Ord α] := BEqCmp (α := α) compare
+
+/-- `LTOrd α` asserts that the `Ord` instance satisfies `LTCmp`. -/
+abbrev LTOrd (α) [LT α] [Ord α] := LTCmp (α := α) compare
+
+/-- `LEOrd α` asserts that the `Ord` instance satisfies `LECmp`. -/
+abbrev LEOrd (α) [LE α] [Ord α] := LECmp (α := α) compare
+
+/-- `LawfulOrd α` asserts that the `Ord` instance satisfies `LawfulCmp`. -/
+abbrev LawfulOrd (α) [LE α] [LT α] [BEq α] [Ord α] := LawfulCmp (α := α) compare
+
+theorem compareOfLessAndEq_eq_lt {x y : α} [LT α] [Decidable (x < y)] [DecidableEq α] :
+    compareOfLessAndEq x y = .lt ↔ x < y := by
+  simp [compareOfLessAndEq]
+  split <;> simpa using Decidable.not_not
+
+protected theorem TransCmp.compareOfLessAndEq
+    [LT α] [DecidableRel (LT.lt (α := α))] [DecidableEq α]
+    (lt_irrefl : ∀ x : α, ¬x < x)
+    (lt_trans : ∀ {x y z : α}, x < y → y < z → x < z)
+    (lt_antisymm : ∀ {x y : α}, ¬x < y → ¬y < x → x = y) :
+    TransCmp (α := α) (compareOfLessAndEq · ·) := by
+  have : OrientedCmp (α := α) (compareOfLessAndEq · ·) := by
+    refine { symm := fun x y => ?_ }
+    simp [compareOfLessAndEq]; split <;> [rename_i xy; split <;> [subst y; rename_i xy ne]]
+    · rw [if_neg, if_neg]; rfl
+      · rintro rfl; exact lt_irrefl _ xy
+      · exact fun yx => lt_irrefl _ (lt_trans xy yx)
+    · rw [if_neg ‹_›, if_pos rfl]; rfl
+    · split <;> [rfl; rename_i yx]
+      cases ne (lt_antisymm xy yx)
+  refine { this with le_trans := fun {x y z} yx zy => ?_ }
+  rw [Ne, this.cmp_eq_gt, compareOfLessAndEq_eq_lt] at yx zy ⊢
+  intro zx
+  if xy : x < y then exact zy (lt_trans zx xy)
+  else exact zy (lt_antisymm yx xy ▸ zx)
+
+protected theorem TransCmp.compareOfLessAndEq_of_le
+    [LT α] [LE α] [DecidableRel (LT.lt (α := α))] [DecidableEq α]
+    (lt_irrefl : ∀ x : α, ¬x < x)
+    (lt_trans : ∀ {x y z : α}, x < y → y < z → x < z)
+    (not_lt : ∀ {x y : α}, ¬x < y → y ≤ x)
+    (le_antisymm : ∀ {x y : α}, x ≤ y → y ≤ x → x = y) :
+    TransCmp (α := α) (compareOfLessAndEq · ·) :=
+  .compareOfLessAndEq lt_irrefl lt_trans fun xy yx => le_antisymm (not_lt yx) (not_lt xy)
+
+protected theorem BEqCmp.compareOfLessAndEq
+    [LT α] [DecidableRel (LT.lt (α := α))] [DecidableEq α] [BEq α] [LawfulBEq α]
+    (lt_irrefl : ∀ x : α, ¬x < x) :
+    BEqCmp (α := α) (compareOfLessAndEq · ·) where
+  cmp_iff_beq {x y} := by
+    simp [compareOfLessAndEq]
+    split <;> [skip; split] <;> simp [*]
+    rintro rfl; exact lt_irrefl _ ‹_›
+
+protected theorem LTCmp.compareOfLessAndEq
+    [LT α] [DecidableRel (LT.lt (α := α))] [DecidableEq α]
+    (lt_irrefl : ∀ x : α, ¬x < x)
+    (lt_trans : ∀ {x y z : α}, x < y → y < z → x < z)
+    (lt_antisymm : ∀ {x y : α}, ¬x < y → ¬y < x → x = y) :
+    LTCmp (α := α) (compareOfLessAndEq · ·) :=
+  { TransCmp.compareOfLessAndEq lt_irrefl lt_trans lt_antisymm with
+    cmp_iff_lt := compareOfLessAndEq_eq_lt }
+
+protected theorem LTCmp.compareOfLessAndEq_of_le
+    [LT α] [DecidableRel (LT.lt (α := α))] [DecidableEq α] [LE α]
+    (lt_irrefl : ∀ x : α, ¬x < x)
+    (lt_trans : ∀ {x y z : α}, x < y → y < z → x < z)
+    (not_lt : ∀ {x y : α}, ¬x < y → y ≤ x)
+    (le_antisymm : ∀ {x y : α}, x ≤ y → y ≤ x → x = y) :
+    LTCmp (α := α) (compareOfLessAndEq · ·) :=
+  { TransCmp.compareOfLessAndEq_of_le lt_irrefl lt_trans not_lt le_antisymm with
+    cmp_iff_lt := compareOfLessAndEq_eq_lt }
+
+protected theorem LECmp.compareOfLessAndEq
+    [LT α] [DecidableRel (LT.lt (α := α))] [DecidableEq α] [LE α]
+    (lt_irrefl : ∀ x : α, ¬x < x)
+    (lt_trans : ∀ {x y z : α}, x < y → y < z → x < z)
+    (not_lt : ∀ {x y : α}, ¬x < y ↔ y ≤ x)
+    (le_antisymm : ∀ {x y : α}, x ≤ y → y ≤ x → x = y) :
+    LECmp (α := α) (compareOfLessAndEq · ·) :=
+  have := TransCmp.compareOfLessAndEq_of_le lt_irrefl lt_trans not_lt.1 le_antisymm
+  { this with
+    cmp_iff_le := (this.cmp_ne_gt).trans <| (not_congr compareOfLessAndEq_eq_lt).trans not_lt }
+
+protected theorem LawfulCmp.compareOfLessAndEq
+    [LT α] [DecidableRel (LT.lt (α := α))] [DecidableEq α] [BEq α] [LawfulBEq α] [LE α]
+    (lt_irrefl : ∀ x : α, ¬x < x)
+    (lt_trans : ∀ {x y z : α}, x < y → y < z → x < z)
+    (not_lt : ∀ {x y : α}, ¬x < y ↔ y ≤ x)
+    (le_antisymm : ∀ {x y : α}, x ≤ y → y ≤ x → x = y) :
+    LawfulCmp (α := α) (compareOfLessAndEq · ·) :=
+  { TransCmp.compareOfLessAndEq_of_le lt_irrefl lt_trans not_lt.1 le_antisymm,
+    LTCmp.compareOfLessAndEq_of_le lt_irrefl lt_trans not_lt.1 le_antisymm,
+    LECmp.compareOfLessAndEq lt_irrefl lt_trans not_lt le_antisymm,
+    BEqCmp.compareOfLessAndEq lt_irrefl with }
+
+theorem LTCmp.eq_compareOfLessAndEq
+    [LT α] [DecidableEq α] [BEq α] [LawfulBEq α] [BEqCmp cmp] [LTCmp cmp]
+    (x y : α) [Decidable (x < y)] : cmp x y = compareOfLessAndEq x y := by
+  simp [compareOfLessAndEq]
+  split <;> rename_i h1 <;> [skip; split <;> rename_i h2]
+  · exact LTCmp.cmp_iff_lt.2 h1
+  · exact BEqCmp.cmp_iff_eq.2 h2
+  · cases e : cmp x y
+    · cases h1 (LTCmp.cmp_iff_lt.1 e)
+    · cases h2 (BEqCmp.cmp_iff_eq.1 e)
+    · rfl
+
+instance [inst₁ : OrientedCmp cmp₁] [inst₂ : OrientedCmp cmp₂] :
+    OrientedCmp (compareLex cmp₁ cmp₂) where
+  symm _ _ := by simp [compareLex, Ordering.swap_then]; rw [inst₁.symm, inst₂.symm]
+
+instance [inst₁ : TransCmp cmp₁] [inst₂ : TransCmp cmp₂] :
+    TransCmp (compareLex cmp₁ cmp₂) where
+  le_trans {a b c} h1 h2 := by
+    simp only [compareLex, ne_eq, Ordering.then_eq_gt, not_or, not_and] at h1 h2 ⊢
+    refine ⟨inst₁.le_trans h1.1 h2.1, fun e1 e2 => ?_⟩
+    match ab : cmp₁ a b with
+    | .gt => exact h1.1 ab
+    | .eq => exact inst₂.le_trans (h1.2 ab) (h2.2 (inst₁.cmp_congr_left ab ▸ e1)) e2
+    | .lt => exact h2.1 <| (inst₁.cmp_eq_gt).2 (inst₁.cmp_congr_left e1 ▸ ab)
+
+instance [Ord β] [inst : OrientedOrd β] (f : α → β) : OrientedCmp (compareOn f) where
+  symm _ _ := OrientedCmp.symm (α := β) ..
+
+instance [Ord β] [inst : TransOrd β] (f : α → β) : TransCmp (compareOn f) where
+  le_trans := TransCmp.le_trans (α := β)
+
+-- FIXME: remove after lean4#3882 is merged
+theorem _root_.lexOrd_def [Ord α] [Ord β] :
+    (lexOrd : Ord (α × β)).compare = compareLex (compareOn (·.1)) (compareOn (·.2)) := by
+  funext a b
+  simp [lexOrd, compareLex, compareOn]; cases compare a.1 b.1 <;> simp [Ordering.then]
+
+section «non-canonical instances»
+-- Note: the following instances seem to cause lean to fail, see:
+-- https://leanprover.zulipchat.com/#narrow/stream/270676-lean4/topic/Typeclass.20inference.20crashes/near/432836360
+
+/-- Local instance for `OrientedOrd lexOrd`. -/
+theorem OrientedOrd.instLexOrd [Ord α] [Ord β]
+    [OrientedOrd α] [OrientedOrd β] : @OrientedOrd (α × β) lexOrd := by
+  rw [OrientedOrd, lexOrd_def]; infer_instance
+
+/-- Local instance for `TransOrd lexOrd`. -/
+theorem TransOrd.instLexOrd [Ord α] [Ord β]
+    [TransOrd α] [TransOrd β] : @TransOrd (α × β) lexOrd := by
+  rw [TransOrd, lexOrd_def]; infer_instance
+
+/-- Local instance for `OrientedOrd ord.opposite`. -/
+theorem OrientedOrd.instOpposite [ord : Ord α] [inst : OrientedOrd α] :
+    @OrientedOrd _ ord.opposite where symm _ _ := inst.symm ..
+
+/-- Local instance for `TransOrd ord.opposite`. -/
+theorem TransOrd.instOpposite [ord : Ord α] [inst : TransOrd α] : @TransOrd _ ord.opposite :=
+  { OrientedOrd.instOpposite with le_trans := fun h1 h2 => inst.le_trans h2 h1 }
+
+/-- Local instance for `OrientedOrd (ord.on f)`. -/
+theorem OrientedOrd.instOn [ord : Ord β] [OrientedOrd β] (f : α → β) : @OrientedOrd _ (ord.on f) :=
+  inferInstanceAs (@OrientedCmp _ (compareOn f))
+
+/-- Local instance for `TransOrd (ord.on f)`. -/
+theorem TransOrd.instOn [ord : Ord β] [TransOrd β] (f : α → β) : @TransOrd _ (ord.on f) :=
+  inferInstanceAs (@TransCmp _ (compareOn f))
+
+/-- Local instance for `OrientedOrd (oα.lex oβ)`. -/
+theorem OrientedOrd.instOrdLex [oα : Ord α] [oβ : Ord β] [OrientedOrd α] [OrientedOrd β] :
+    @OrientedOrd _ (oα.lex oβ) := OrientedOrd.instLexOrd
+
+/-- Local instance for `TransOrd (oα.lex oβ)`. -/
+theorem TransOrd.instOrdLex [oα : Ord α] [oβ : Ord β] [TransOrd α] [TransOrd β] :
+    @TransOrd _ (oα.lex oβ) := TransOrd.instLexOrd
+
+/-- Local instance for `OrientedOrd (oα.lex' oβ)`. -/
+theorem OrientedOrd.instOrdLex' (ord₁ ord₂ : Ord α) [@OrientedOrd _ ord₁] [@OrientedOrd _ ord₂] :
+    @OrientedOrd _ (ord₁.lex' ord₂) :=
+  inferInstanceAs (OrientedCmp (compareLex ord₁.compare ord₂.compare))
+
+/-- Local instance for `TransOrd (oα.lex' oβ)`. -/
+theorem TransOrd.instOrdLex' (ord₁ ord₂ : Ord α) [@TransOrd _ ord₁] [@TransOrd _ ord₂] :
+    @TransOrd _ (ord₁.lex' ord₂) :=
+  inferInstanceAs (TransCmp (compareLex ord₁.compare ord₂.compare))
+
+end «non-canonical instances»
+
+instance : LawfulOrd Nat := .compareOfLessAndEq
+  Nat.lt_irrefl Nat.lt_trans Nat.not_lt Nat.le_antisymm
+
+instance : LawfulOrd (Fin n) where
+  symm _ _ := OrientedCmp.symm (α := Nat) (cmp := compare) ..
+  le_trans := TransCmp.le_trans (α := Nat) (cmp := compare)
+  cmp_iff_beq := (BEqCmp.cmp_iff_beq (α := Nat) (cmp := compare)).trans (by simp [Fin.ext_iff])
+  cmp_iff_lt := LTCmp.cmp_iff_lt (α := Nat) (cmp := compare)
+  cmp_iff_le := LECmp.cmp_iff_le (α := Nat) (cmp := compare)
+
+instance : LawfulOrd Bool where
+  symm := by decide
+  le_trans := by decide
+  cmp_iff_beq := by decide
+  cmp_iff_lt := by decide
+  cmp_iff_le := by decide
+
+instance : LawfulOrd Int := .compareOfLessAndEq
+  Int.lt_irrefl Int.lt_trans Int.not_lt Int.le_antisymm
+
 end Std
 
 namespace Ordering
@@ -105,9 +365,6 @@ open Std
 
 instance (f : α → β) (cmp : β → β → Ordering) [OrientedCmp cmp] : OrientedCmp (byKey f cmp) where
   symm a b := OrientedCmp.symm (f a) (f b)
-
-instance (f : α → β) (cmp : β → β → Ordering) [TransCmp cmp] : TransCmp (byKey f cmp) where
-  le_trans h₁ h₂ := TransCmp.le_trans (α := β) h₁ h₂
 
 instance (f : α → β) (cmp : β → β → Ordering) [TransCmp cmp] : TransCmp (byKey f cmp) where
   le_trans h₁ h₂ := TransCmp.le_trans (α := β) h₁ h₂
