Std/Data/UInt.lean
@@ -1,13 +1,16 @@
 /-
 Copyright (c) 2023 François G. Dorais. All rights reserved.
 Released under Apache 2.0 license as described in the file LICENSE.
-Authors: François G. Dorais
+Authors: François G. Dorais, Mario Carneiro
 -/
+import Std.Classes.Order
 
 /-! ### UInt8 -/
 
 @[ext] theorem UInt8.ext : {x y : UInt8} → x.toNat = y.toNat → x = y
   | ⟨⟨_,_⟩⟩, ⟨⟨_,_⟩⟩, rfl => rfl
+
+theorem UInt8.ext_iff {x y : UInt8} : x = y ↔ x.toNat = y.toNat := ⟨congrArg _, UInt8.ext⟩
 
 @[simp] theorem UInt8.val_val_eq_toNat (x : UInt8) : x.val.val = x.toNat := rfl
 
@@ -22,10 +25,21 @@ theorem UInt8.toNat_lt (x : UInt8) : x.toNat < 2 ^ 8 := x.val.isLt
 @[simp] theorem UInt8.toUInt64_toNat (x : UInt8) : x.toUInt64.toNat = x.toNat :=
   Nat.mod_eq_of_lt (Nat.lt_of_lt_of_le x.toNat_lt (by decide))
 
+theorem UInt8.le_antisymm_iff {x y : UInt8} : x = y ↔ x ≤ y ∧ y ≤ x :=
+  UInt8.ext_iff.trans Nat.le_antisymm_iff
+
+theorem UInt8.le_antisymm {x y : UInt8} (h1 : x ≤ y) (h2 : y ≤ x) : x = y :=
+  UInt8.le_antisymm_iff.2 ⟨h1, h2⟩
+
+instance : Std.LawfulOrd UInt8 := .compareOfLessAndEq
+  (fun _ => Nat.lt_irrefl _) Nat.lt_trans Nat.not_lt UInt8.le_antisymm
+
 /-! ### UInt16 -/
 
 @[ext] theorem UInt16.ext : {x y : UInt16} → x.toNat = y.toNat → x = y
   | ⟨⟨_,_⟩⟩, ⟨⟨_,_⟩⟩, rfl => rfl
+
+theorem UInt16.ext_iff {x y : UInt16} : x = y ↔ x.toNat = y.toNat := ⟨congrArg _, UInt16.ext⟩
 
 theorem UInt16.toNat_lt (x : UInt16) : x.toNat < 2 ^ 16 := x.val.isLt
 
@@ -39,10 +53,21 @@ theorem UInt16.toNat_lt (x : UInt16) : x.toNat < 2 ^ 16 := x.val.isLt
 @[simp] theorem UInt16.toUInt64_toNat (x : UInt16) : x.toUInt64.toNat = x.toNat :=
   Nat.mod_eq_of_lt (Nat.lt_of_lt_of_le x.toNat_lt (by decide))
 
+theorem UInt16.le_antisymm_iff {x y : UInt16} : x = y ↔ x ≤ y ∧ y ≤ x :=
+  UInt16.ext_iff.trans Nat.le_antisymm_iff
+
+theorem UInt16.le_antisymm {x y : UInt16} (h1 : x ≤ y) (h2 : y ≤ x) : x = y :=
+  UInt16.le_antisymm_iff.2 ⟨h1, h2⟩
+
+instance : Std.LawfulOrd UInt16 := .compareOfLessAndEq
+  (fun _ => Nat.lt_irrefl _) Nat.lt_trans Nat.not_lt UInt16.le_antisymm
+
 /-! ### UInt32 -/
 
 @[ext] theorem UInt32.ext : {x y : UInt32} → x.toNat = y.toNat → x = y
   | ⟨⟨_,_⟩⟩, ⟨⟨_,_⟩⟩, rfl => rfl
+
+theorem UInt32.ext_iff {x y : UInt32} : x = y ↔ x.toNat = y.toNat := ⟨congrArg _, UInt32.ext⟩
 
 @[simp] theorem UInt32.val_val_eq_toNat (x : UInt32) : x.val.val = x.toNat := rfl
 
@@ -55,10 +80,21 @@ theorem UInt32.toNat_lt (x : UInt32) : x.toNat < 2 ^ 32 := x.val.isLt
 @[simp] theorem UInt32.toUInt64_toNat (x : UInt32) : x.toUInt64.toNat = x.toNat :=
   Nat.mod_eq_of_lt (Nat.lt_of_lt_of_le x.toNat_lt (by decide))
 
+theorem UInt32.le_antisymm_iff {x y : UInt32} : x = y ↔ x ≤ y ∧ y ≤ x :=
+  UInt32.ext_iff.trans Nat.le_antisymm_iff
+
+theorem UInt32.le_antisymm {x y : UInt32} (h1 : x ≤ y) (h2 : y ≤ x) : x = y :=
+  UInt32.le_antisymm_iff.2 ⟨h1, h2⟩
+
+instance : Std.LawfulOrd UInt32 := .compareOfLessAndEq
+  (fun _ => Nat.lt_irrefl _) Nat.lt_trans Nat.not_lt UInt32.le_antisymm
+
 /-! ### UInt64 -/
 
 @[ext] theorem UInt64.ext : {x y : UInt64} → x.toNat = y.toNat → x = y
   | ⟨⟨_,_⟩⟩, ⟨⟨_,_⟩⟩, rfl => rfl
+
+theorem UInt64.ext_iff {x y : UInt64} : x = y ↔ x.toNat = y.toNat := ⟨congrArg _, UInt64.ext⟩
 
 @[simp] theorem UInt64.val_val_eq_toNat (x : UInt64) : x.val.val = x.toNat := rfl
 
@@ -70,10 +106,21 @@ theorem UInt64.toNat_lt (x : UInt64) : x.toNat < 2 ^ 64 := x.val.isLt
 
 @[simp] theorem UInt64.toUInt32_toNat (x : UInt64) : x.toUInt32.toNat = x.toNat % 2 ^ 32 := rfl
 
+theorem UInt64.le_antisymm_iff {x y : UInt64} : x = y ↔ x ≤ y ∧ y ≤ x :=
+  UInt64.ext_iff.trans Nat.le_antisymm_iff
+
+theorem UInt64.le_antisymm {x y : UInt64} (h1 : x ≤ y) (h2 : y ≤ x) : x = y :=
+  UInt64.le_antisymm_iff.2 ⟨h1, h2⟩
+
+instance : Std.LawfulOrd UInt64 := .compareOfLessAndEq
+  (fun _ => Nat.lt_irrefl _) Nat.lt_trans Nat.not_lt UInt64.le_antisymm
+
 /-! ### USize -/
 
 @[ext] theorem USize.ext : {x y : USize} → x.toNat = y.toNat → x = y
   | ⟨⟨_,_⟩⟩, ⟨⟨_,_⟩⟩, rfl => rfl
+
+theorem USize.ext_iff {x y : USize} : x = y ↔ x.toNat = y.toNat := ⟨congrArg _, USize.ext⟩
 
 @[simp] theorem USize.val_val_eq_toNat (x : USize) : x.val.val = x.toNat := rfl
 
@@ -99,3 +146,12 @@ theorem USize.toNat_lt (x : USize) : x.toNat < 2 ^ System.Platform.numBits := by
 
 @[simp] theorem UInt32.toUSize_toNat (x : UInt32) : x.toUSize.toNat = x.toNat :=
   Nat.mod_eq_of_lt (Nat.lt_of_lt_of_le x.toNat_lt USize.le_size)
+
+theorem USize.le_antisymm_iff {x y : USize} : x = y ↔ x ≤ y ∧ y ≤ x :=
+  USize.ext_iff.trans Nat.le_antisymm_iff
+
+theorem USize.le_antisymm {x y : USize} (h1 : x ≤ y) (h2 : y ≤ x) : x = y :=
+  USize.le_antisymm_iff.2 ⟨h1, h2⟩
+
+instance : Std.LawfulOrd USize := .compareOfLessAndEq
+  (fun _ => Nat.lt_irrefl _) Nat.lt_trans Nat.not_lt USize.le_antisymm
